Add partial implementation for analyzing add_num.dfy

dafny/src/interpreter.dfy
@@ -1,11 +1,15 @@
 include "BoundedInts.dfy"
 include "types.dfy"
 include "ebpf.dfy"
+include "helpers.dfy"
 
 module eBPFInterpreter {
   import opened BoundedInts
   import opened parser
   import opened types
+  import opened helpers
+
+  const BPF_MAX_REG := 11
 
   function RegisterToInt(reg: RegisterOrUnused): uint8
   {
@@ -71,8 +75,58 @@ module eBPFInterpreter {
     ret
   }
 
-  function checkRegArg(env: BPFVerifierEnv, reg: RegisterOrUnused, argType: RegisterArgType): bool {
-    false
+  //TODO: Fill in all the cases
+  function isReg64(env: BPFVerifierEnv, instruction: Statement, register: RegisterOrUnused, regstate: BPFRegState, argType: RegisterArgType): bool
+    requires instruction.Instruction?
+    requires !register.UNUSED?
+  {
+    match instruction.op {
+      case JumpOperation(jumpInstructionClass, jumpSource, jumpOpcode) =>
+        if jumpOpcode == BPF_EXIT then
+          true
+        else if jumpOpcode == BPF_CALL then
+          // BPF Pseudo Call
+          if RegisterToInt(instruction.srcReg) == 0x1 then
+            false
+          else if argType == SRC_OP then
+            true
+          else
+            false
+        else
+          true
+
+
+      case ArithmeticOperation(arithmeticInstructionClass, arithSource, arithOpcode) =>
+        if arithmeticInstructionClass == ArithmeticInstructionClass.BPF_ALU64 then
+          true
+        else
+          false
+
+      case default => false
+    }
+  }
+
+  function checkRegArg(env: BPFVerifierEnv, instruction: Statement, reg: RegisterOrUnused, argType: RegisterArgType): bool
+    requires instruction.Instruction?
+    requires !reg.UNUSED?
+    requires env.cur_state.curframe as int < |env.cur_state.frame|
+    requires |curRegs(env)| == BPF_MAX_REG
+  {
+    //TODO: Mark register scratched, maybe not very important
+    var regState := curRegs(env)[RegisterToInt(reg)];
+    var is64 := isReg64(env, instruction, reg, regState, argType);
+    if argType == SRC_OP then
+      //TODO: Fill in this case
+      true
+    else
+    // Frame Pointer is read only
+    if reg == RegisterOrUnused.R10 then
+      //TODO: Add an error code here
+      false
+    else
+      //TODO: The
+      true
+
   }
 
   predicate check_mem_access(env: BPFVerifierEnv, insn_idx: uint32, register: RegisterOrUnused,
@@ -80,14 +134,131 @@ module eBPFInterpreter {
     true
   }
 
-  function cur_regs(env: BPFVerifierEnv): seq<BPFRegState>
+  function curRegs(env: BPFVerifierEnv): seq<BPFRegState>
     requires env.cur_state.BPFVerifierState?
     requires env.cur_state.curframe as int < |env.cur_state.frame|
   {
     env.cur_state.frame[env.cur_state.curframe].regs
   }
 
+  function frameRegs(env: BPFVerifierEnv, frameno: uint32): seq<BPFRegState>
+    requires env.cur_state.BPFVerifierState?
+    requires frameno as int < |env.cur_state.frame|
+  {
+    env.cur_state.frame[frameno].regs
+  }
+
+  function update_regs(env: BPFVerifierEnv, regstate: BPFRegState, regno: uint8, frameno: uint32): BPFVerifierEnv
+    requires frameno as int < |env.cur_state.frame|
+    requires env.cur_state.curframe as int < |env.cur_state.frame|
+    requires |frameRegs(env, frameno)| == BPF_MAX_REG
+    requires 0 <= regno < BPF_MAX_REG as uint8
+  {
+    var frame_regs:= env.cur_state.frame[frameno].regs;
+    var new_regs := frame_regs[regno := regstate];
+    var new_func_state := env.cur_state.frame[frameno].(regs := new_regs);
+    var new_frames := env.cur_state.(frame := env.cur_state.frame[frameno := new_func_state]);
+    env.(cur_state := new_frames)
+  }
+
+  function markRegUnbounded(reg: BPFRegState): BPFRegState {
+    reg.(smin_value := S64_MIN, smax_value := S64_MAX, umin_value := U64_MIN, umax_value := U64_MAX,
+    s32_min_value := S32_MIN, s32_max_value := S32_MAX, u32_min_value := U32_MIN, u32_max_value := U32_MAX)
+  }
+
+  function markRegUnknown(env: BPFVerifierEnv, regs: seq<BPFRegState>, reg: RegisterOrUnused): BPFVerifierEnv
+    requires |regs| == BPF_MAX_REG
+    requires env.cur_state.curframe as int < |env.cur_state.frame|
+    requires |regs| == BPF_MAX_REG
+    requires |curRegs(env)| == BPF_MAX_REG
+  {
+    var regno := RegisterToInt(reg);
+    //TODO: Model and clear the union data in the kernel regstate
+    //TODO: Model the ref_obj_id and precise fields
+    var regstate := regs[regno].(typ := SCALAR_VALUE, offset := 0, id := 0, var_off := TristateNum(0, U64_MAX as uint64), frameno := 0);
+    var regstate := markRegUnbounded(regstate);
+    //TODO: Mark all fields appropriately
+
+    update_regs(env, regstate, regno, env.cur_state.curframe)
+  }
+
+  function markRegKnown___(reg: BPFRegState, imm: int32): BPFRegState {
+    reg.(smin_value := imm as int64, smax_value := imm as int64, umin_value := signed32_to_unsigned64(imm), umax_value := signed32_to_unsigned64(imm),
+    s32_min_value := imm, s32_max_value := imm, u32_min_value := signed32_to_unsigned32(imm), u32_max_value := signed32_to_unsigned32(imm))
+  }
+
+  function markRegKnown__(env: BPFVerifierEnv, regs: seq<BPFRegState>, reg: RegisterOrUnused, imm: int32): BPFVerifierEnv
+    requires env.cur_state.curframe as int < |env.cur_state.frame|
+    requires |regs| == BPF_MAX_REG
+    requires |curRegs(env)| == BPF_MAX_REG
+  {
+    var regno := RegisterToInt(reg);
+    //TODO: Model the union in struct bpf_reg_state
+    //TODO: Model the ref_obj_id
+    var regstate := regs[regno].(offset := 0, id := 0);
+    var regstate := markRegKnown___(regstate, imm);
+
+    update_regs(env, regstate, regno, env.cur_state.curframe)
+  }
+
+  function adjustRegMinMaxVals(env: BPFVerifierEnv, instruction: Statement): (BPFVerifierEnv, Error) {
+    //TODO: Implement this
+    (env, Success)
+  }
+ 
+
+  function handleALUOp(instruction: Statement, env: BPFVerifierEnv): (BPFVerifierEnv, Error)
+    requires instruction.Instruction?
+    requires instruction.op.ArithmeticOperation?
+    requires env.cur_state.curframe as int < |env.cur_state.frame|
+    requires |curRegs(env)| == BPF_MAX_REG
+    requires instruction.op.arithmeticOpcode == BPF_MOV ==> !instruction.destReg.UNUSED?
+    requires instruction.op.arithmeticOpcode == ArithmeticOpCode.BPF_ADD ==> !instruction.destReg.UNUSED?
+  {
+    var srcReg: RegisterOrUnused := instruction.srcReg;
+    var destReg: RegisterOrUnused := instruction.destReg;
+
+    var op := instruction.op.arithmeticOpcode;
+
+    var t := match instruction.op.arithmeticOpcode {
+      case BPF_MOV =>
+        //TODO: do checks for reserved fields
+        var err := checkRegArg(env, instruction, instruction.destReg, DST_OP_NO_MARK);
+        //TODO: Do early return on error here
+        match instruction.op.arithmeticSource {
+          // R = dest
+          case BPF_X => (env, Success)
+          // R = imm
+          case BPF_K =>
+            var temp_env := markRegUnknown(env, curRegs(env), instruction.destReg);
+            var dest_reg_state := curRegs(temp_env)[RegisterToInt(instruction.destReg)];
+            // Question: How does multiple declarations work here?
+            var temp_env := update_regs(temp_env, dest_reg_state.(typ := SCALAR_VALUE), RegisterToInt(instruction.destReg), temp_env.cur_state.curframe);
+            //TODO: Mark reg as known with the immediate
+            var temp_env := markRegKnown__(env, curRegs(env), instruction.destReg, instruction.immediate);
+            (temp_env, Success)
+        }
+
+      case BPF_ADD => 
+        //TODO: do checks for reserved fields
+        var err := checkRegArg(env, instruction, instruction.destReg, SRC_OP);
+        //TODO: Do early return on error here
+        //TODO: do more checks
+        var err := checkRegArg(env, instruction, instruction.destReg, DST_OP_NO_MARK);
+        //TODO: Do early return on error here
+        adjustRegMinMaxVals(env, instruction)
+        
+
+      case default => (env, Success)
+    };
+
+    t
+
+    //(env, Success)
+  }
+
   // Assumes that the program has just a single global function
+  // Assumes that there are no Immediate32 in the instruction stream
   method runVerifier(program: BPFProg) returns (valid: bool)
     requires |program.prog.s| > 0
     requires forall idx :: 0 <= idx < |program.prog.s| ==> program.prog.s[idx].Instruction?
@@ -126,14 +297,34 @@ module eBPFInterpreter {
 
             var srcRegNo := RegisterToInt(instruction.srcReg);
 
+            // Logically this is an error, UNUSED is treated as R0
+            // If this condition is true then it indicates an error in the assembly parser
+            if instruction.srcReg.UNUSED? {
+              return false;
+            }
+
             // Question: How to update nested structs in a better way?
-            err := checkRegArg(env, instruction.srcReg, SRC_OP) || checkRegArg(env, instruction.destReg, DST_OP_NO_MARK) ||
+            err := checkRegArg(env, instruction, instruction.srcReg, SRC_OP) || checkRegArg(env, instruction, instruction.destReg, DST_OP_NO_MARK) ||
                    check_mem_access(env, env.insn_idx, instruction.srcReg,
                                     instruction.offset, loadSize, BPF_READ, instruction.destReg, false); // Checks memory access and updates the abstract state of the register
 
             //TODO: Implement AUX ptr type
             //err := err || saveAuxPtrType(env, cur_regs(env)[srcRegNo], false);
           }
+        }
+
+        case ArithmeticOperation(arithInstructionClass, arithSrc, arithOp) => {
+          if arithInstructionClass == ArithmeticInstructionClass.BPF_ALU64 ||
+             arithInstructionClass == ArithmeticInstructionClass.BPF_ALU {
+            if !instruction.destReg.UNUSED? {
+              // Question: How to handle multiple returns?
+              var r := handleALUOp(instruction, env);
+            } else {
+              print "BPF_MOV has dest reg UNUSED";
+            }
+
+          }
+
         }
 
         case default => {}
