dafny/src/examples/add_num.dfy
@@ -8,20 +8,20 @@
 */
 
 module add_example {
-    import opened parser
+  import opened parser
 
-    function add_example(): BPFProgram {
-        var statement00Op: Op := ArithmeticOperation(ArithmeticInstructionClass.BPF_ALU64, ArithmeticSource.BPF_K, ArithmeticOpCode.BPF_MOV);
-        var statement00: Statement := Instruction(statement00Op, RegisterOrUnused.UNUSED, RegisterOrUnused.R0, 0x0, 0x01);
+  function add_example(): BPFProgram {
+    var statement00Op: Op := ArithmeticOperation(ArithmeticInstructionClass.BPF_ALU64, ArithmeticSource.BPF_K, ArithmeticOpCode.BPF_MOV);
+    var statement00: Statement := Instruction(statement00Op, RegisterOrUnused.UNUSED, RegisterOrUnused.R0, 0x0, 0x01);
 
-        var statement01Op: Op := ArithmeticOperation(ArithmeticInstructionClass.BPF_ALU64, ArithmeticSource.BPF_K, ArithmeticOpCode.BPF_ADD);
-        var statement01: Statement := Instruction(statement01Op, RegisterOrUnused.UNUSED, RegisterOrUnused.R0, 0x0, 0x2);
+    var statement01Op: Op := ArithmeticOperation(ArithmeticInstructionClass.BPF_ALU64, ArithmeticSource.BPF_K, ArithmeticOpCode.BPF_ADD);
+    var statement01: Statement := Instruction(statement01Op, RegisterOrUnused.UNUSED, RegisterOrUnused.R0, 0x0, 0x2);
 
-        var statement02Op: Op := JumpOperation(JumpInstructionClass.BPF_JMP, JumpSource.BPF_K, JumpOpCode.BPF_EXIT);
-        var statement02 : Statement := Instruction(statement02Op, RegisterOrUnused.UNUSED, RegisterOrUnused.UNUSED, 0x0, 0x0);
+    var statement02Op: Op := JumpOperation(JumpInstructionClass.BPF_JMP, JumpSource.BPF_K, JumpOpCode.BPF_EXIT);
+    var statement02 : Statement := Instruction(statement02Op, RegisterOrUnused.UNUSED, RegisterOrUnused.UNUSED, 0x0, 0x0);
 
-        var stmt_seq: seq<Statement> := [statement00, statement01, statement02];
+    var stmt_seq: seq<Statement> := [statement00, statement01, statement02];
 
-        Statements(stmt_seq)
-    }
+    Statements(stmt_seq)
+  }
 }
